@base <http://www.dotnetrdf.org/optimiserStats#> .

@prefix rdf: <http://www.w3.org/1999/02/22-rdf-syntax-ns#>.
@prefix rdfs: <http://www.w3.org/2000/01/rdf-schema#>.
@prefix xsd: <http://www.w3.org/2001/XMLSchema#>.
@prefix opt: <http://www.dotnetrdf.org/optimiserStats#> .

opt:count a rdf:Property ;
		   rdfs:label "Count" ;
		   rdfs:comment "Gives the estimated count of occurrences of a RDF term, specifying this for a term is equivalent to specifying opt:subjectCount, opt:predicateCount and opt:objectCount.  Weighting of Terms is proportional to the count i.e. the higher the count the less selective a term is considered to be" ;
		   rdfs:range xsd:integer .
		   
opt:subjectCount a rdf:Property ;
				   rdfs:label "Subject Count" ;
				   rdfs:comment "Gives the estimated count of occurrences of a RDF term in the subject position." ;
				   rdfs:range xsd:integer .
				   
opt:predicateCount a rdf:Property ;
				     rdfs:label "Predicate Count" ;
				     rdfs:comment "Gives the estimated count of occurrences of a RDF term in the predicate position." ;
				     rdfs:range xsd:integer .
				   
opt:objectCount a rdf:Property ;
				  rdfs:label "Object Count" ;
				  rdfs:comment "Gives the estimated count of occurrences of a RDF term in the object position." ;
				  rdfs:range xsd:integer .